implement agent protocols

paxos/agents.dfy
@@ -8,21 +8,27 @@ import opened Types
 *                                Acceptor State Machine                                  *
 *****************************************************************************************/
 
-datatype Acceptor = Acceptor(id:Id, promised:Ballot, accepted:Value)
+datatype AcceptorConstants = AConsts(id:Id)
+
+datatype Acceptor = Acceptor(
+    consts:AcceptorConstants, 
+    promised:Ballot, 
+    accepted:Value)
 
 /* Acceptor initial state */
 predicate AcceptorInit(a:Acceptor, id:Id) {
-    && a.id == id
+    && a.consts == AConsts(id)
     && a.promised == Bottom
     && a.accepted == Nil
 }
 
 /* Acceptor next state */
-predicate AcceptorNext(a:Acceptor, a':Acceptor, recvIo:Packet, sendIo:seq<Packet>) {
-    && a'.id == a.id
-    && match recvIo.msg {
-        case Prepare(bal) => AcceptorNext_RcvPrepare(a, a', recvIo, sendIo)
-        case Propose(bal, val) => AcceptorNext_RcvPropose(a, a', recvIo, sendIo)
+predicate AcceptorNext(a:Acceptor, a':Acceptor, recvIos:seq<Packet>, sendIo:seq<Packet>) {
+    && a'.consts == a.consts
+    && |recvIos| == 1
+    && match recvIos[0].msg {
+        case Prepare(bal) => AcceptorNext_RcvPrepare(a, a', recvIos[0], sendIo)
+        case Propose(bal, val) => AcceptorNext_RcvPropose(a, a', recvIos[0], sendIo)
         case _ => a == a' && sendIo == []
     }
 }
@@ -38,47 +44,48 @@ predicate AcceptorNext_RcvPrepare(a:Acceptor, a':Acceptor, recvIo:Packet, sendIo
 }
 
 /* Acceptor next state, process Accept message */
-predicate AcceptorNext_RcvPropose(a:Acceptor, a':Acceptor, recvIo:Packet, sendIo:seq<Packet>) 
+predicate AcceptorNext_RcvPropose(a:Acceptor, a':Acceptor, recvIo:Packet, sendIos:seq<Packet>) 
     requires recvIo.msg.Propose?
 {
     if BalLtEq(a.promised, recvIo.msg.bal)  then
-        AcceptorAccept(a, a', recvIo, sendIo)
+        AcceptorAccept(a, a', recvIo, sendIos)
     else 
-        AcceptorPreempt(a, a', recvIo, sendIo)
+        AcceptorPreempt(a, a', recvIo, sendIos)
 }
 
 /* Acceptor send Promise */
-predicate AcceptorPromise(a:Acceptor, a':Acceptor, recvIo:Packet, sendIo:seq<Packet>) 
+predicate AcceptorPromise(a:Acceptor, a':Acceptor, recvIo:Packet, sendIos:seq<Packet>) 
     requires recvIo.msg.Prepare?
 {
     && a'.promised == recvIo.msg.bal
     && a'.accepted == a.accepted
-    && |sendIo| == 1
-    && sendIo[0].src == a.id
-    && sendIo[0].dst == recvIo.src
-    && sendIo[0].msg == Promise(a.accepted)
+    && |sendIos| == 1
+    && sendIos[0].src == a.consts.id
+    && sendIos[0].dst == recvIo.src
+    && sendIos[0].msg == Promise(a.promised, a.accepted)
 }
 
 /* Acceptor send Accept */
-predicate AcceptorAccept(a:Acceptor, a':Acceptor, recvIo:Packet, sendIo:seq<Packet>) 
+predicate AcceptorAccept(a:Acceptor, a':Acceptor, recvIo:Packet, sendIos:seq<Packet>) 
     requires recvIo.msg.Propose?
 {
     && a'.promised == recvIo.msg.bal
     && a'.accepted == recvIo.msg.val
-    && |sendIo| == 1
-    && sendIo[0].src == a.id
-    && sendIo[0].dst == recvIo.src
-    && sendIo[0].msg == Accept()
+    && |sendIos| == 1
+    && sendIos[0].src == a.consts.id
+    && sendIos[0].dst == recvIo.src
+    && sendIos[0].msg == Accept(recvIo.msg.bal)
 }
 
 /* Acceptor send Preempt */
-predicate AcceptorPreempt(a:Acceptor, a':Acceptor, recvIo:Packet, sendIo:seq<Packet>) 
+predicate AcceptorPreempt(a:Acceptor, a':Acceptor, recvIo:Packet, sendIos:seq<Packet>) 
     requires recvIo.msg.Prepare? || recvIo.msg.Propose?
 {
-    && |sendIo| == 1
-    && sendIo[0].src == a.id
-    && sendIo[0].dst == recvIo.src
-    && sendIo[0].msg == Preempt(a.promised, a.accepted)
+    && |sendIos| == 1
+    && sendIos[0].src == a.consts.id
+    && sendIos[0].dst == recvIo.src
+    && sendIos[0].msg == Preempt(a.promised, a.accepted)
+    // Bug: a'.promised and a'.accepted unspecified
 }
 
 
@@ -86,21 +93,190 @@ predicate AcceptorPreempt(a:Acceptor, a':Acceptor, recvIo:Packet, sendIo:seq<Pac
 *                                 Leader State Machine                                   *
 *****************************************************************************************/
 
-datatype LeaderState = P1a | P1b | P2a | P2b
+datatype LeaderState = P1a | P1b | P2a | P2b | Decided
+datatype LeaderConstants = LConsts(id:Id, accConf:seq<Id>, f:nat, initval:Value)
 
 datatype Leader = Leader(
-    id:Id,
+    consts:LeaderConstants,    
     state:LeaderState,
     ballot:Ballot,
-    val:Value
+    val:Value,
+    promises:set<Id>,
+    accepts:set<Id>
 )
 
 /* Leader initial state */
-predicate LeaderInit(l:Leader, id:Id) {
-    && l.id == id
+predicate LeaderInit(l:Leader, id:Id, accConf:seq<Id>, f:nat, initval:Value) {
+    && l.consts == LConsts(id, accConf, f, initval)
     && l.state == P1a
     && l.ballot == Ballot(0, id.num)
-    // value to propose is intentionally unspecified
+    && l.val == initval
 }
 
+/* Leader next state */
+predicate LeaderNext(l:Leader, l':Leader, recvIos:seq<Packet>, sendIos:seq<Packet>) {
+    && l'.consts == l.consts
+    && match l.state {
+        case P1a => LeaderNext_P1a(l, l', recvIos, sendIos)
+        case P1b => LeaderNext_P1b(l, l', recvIos, sendIos)
+        case P2a => LeaderNext_P2a(l, l', recvIos, sendIos)
+        case P2b => LeaderNext_P2b(l, l', recvIos, sendIos)
+        case Decided => LeaderStutter(l, l', sendIos)
+    }
+}
+
+
+/* Leader next state, broadcast Prepare messages */
+predicate LeaderNext_P1a(l:Leader, l':Leader, recvIos:seq<Packet>, sendIos:seq<Packet>) 
+    requires l.state == P1a
+{
+    && l'.state == P1b
+    && l'.ballot == l.ballot
+    && l'.val == l.val
+    && l'.promises == l.promises
+    && l'.accepts == l.accepts
+    && recvIos == []
+    && LeaderSendPrepare(l, sendIos)
+}
+
+predicate LeaderSendPrepare(l:Leader, sendIos:seq<Packet>) {
+    && |sendIos| == |l.consts.accConf|
+    && forall i | 0 <= i < |sendIos| 
+        :: sendIos[i] == Packet(l.consts.id, l.consts.accConf[i], Prepare(l.ballot))
+}
+
+
+/* Leader next state, wait for quorum of Promise messages */
+predicate LeaderNext_P1b(l:Leader, l':Leader, recvIos:seq<Packet>, sendIos:seq<Packet>) 
+    requires l.state == P1b
+{
+    && |recvIos| == 1 
+    && match recvIos[0].msg {
+        case Prepare(bal) => LeaderStutter(l, l', sendIos)
+        case Promise(bal, val) => LeaderProcessPromise(l, l', recvIos[0], sendIos)
+        case Propose(bal, val) => LeaderStutter(l, l', sendIos)
+        case Accept(bal) =>  LeaderStutter(l, l', sendIos)
+        case Preempt(bal, val) => LeaderProcessPreempt(l, l', recvIos[0].msg, sendIos)
+    }
+}
+
+predicate LeaderStutter(l:Leader, l':Leader, sendIos:seq<Packet>) {
+    l' == l && sendIos == []
+}
+
+predicate LeaderProcessPromise(l:Leader, l':Leader, pkt:Packet, sendIos:seq<Packet>) 
+    requires pkt.msg.Promise?
+    requires l.state == P1b
+{
+    var src, msg := pkt.src, pkt.msg;
+    if msg.bal == l.ballot && src !in l.promises then
+        LeaderProcessValidPromise(l, l', src, msg, sendIos)
+    else 
+        // This is a stale promise
+        LeaderStutter(l, l', sendIos)
+}
+
+predicate LeaderProcessValidPromise(l:Leader, l':Leader, src:Id, msg:Message, sendIos:seq<Packet>) 
+    requires msg.Promise?
+    requires l.state == P1b
+{
+    if |l.promises| == 2*l.consts.f then 
+        // Go to phase 2a
+        && l'.state == P2a
+        && l'.ballot == l.ballot
+        && l'.val == (if msg.val == Nil then l.val else msg.val)
+        && l'.promises == {}
+        && l'.accepts == {}
+    else 
+        && l'.state == l.state
+        && l'.ballot == l.ballot
+        && l'.val == (if msg.val == Nil then l.val else msg.val)
+        && l'.promises == l.promises + {src}
+        && l'.accepts == l.accepts
+}
+
+predicate LeaderProcessPreempt(l:Leader, l':Leader, msg:Message, sendIos:seq<Packet>) 
+    requires msg.Preempt?
+{
+    if BalLt(l.ballot, msg.bal) then 
+        // I am preempted
+        && l'.state == P1a
+        && l'.ballot == NextBallot(msg.bal, l.consts.id.num)
+        && l'.promises == {}
+        && l'.accepts == {}
+        && if msg.val == Nil 
+            then l'.val == l.val
+            else l'.val == msg.val
+    else 
+        // False alarm, msg is stale
+        LeaderStutter(l, l', sendIos)
+}
+
+
+/* Leader next state, broadcast Propose messages */
+predicate LeaderNext_P2a(l:Leader, l':Leader, recvIos:seq<Packet>, sendIos:seq<Packet>) 
+    requires l.state == P2a
+{
+    && l'.state == P2b
+    && l'.ballot == l.ballot
+    && l'.val == l.val
+    && l'.promises == l.promises
+    && l'.accepts == l.accepts
+    && recvIos == []
+    && LeaderSendPropose(l, sendIos)
+}
+
+predicate LeaderSendPropose(l:Leader, sendIos:seq<Packet>) 
+    requires l.state == P2a
+{
+    && |sendIos| == |l.consts.accConf|
+    && forall i | 0 <= i < |sendIos| 
+        :: sendIos[i] == Packet(l.consts.id, l.consts.accConf[i], Propose(l.ballot, l.val))
+}
+
+
+/* Leader next state, wait for quorum of Accept messages */
+predicate LeaderNext_P2b(l:Leader, l':Leader, recvIos:seq<Packet>, sendIos:seq<Packet>) 
+    requires l.state == P2b
+{
+    && |recvIos| == 1 
+    && match recvIos[0].msg {
+        case Prepare(bal) => LeaderStutter(l, l', sendIos)
+        case Promise(bal, val) => LeaderStutter(l, l', sendIos)
+        case Propose(bal, val) => LeaderStutter(l, l', sendIos)
+        case Accept(bal) =>  LeaderProcessAccept(l, l', recvIos[0], sendIos)
+        case Preempt(bal, val) => LeaderProcessPreempt(l, l', recvIos[0].msg, sendIos)
+    }
+}
+
+predicate LeaderProcessAccept(l:Leader, l':Leader, pkt:Packet, sendIos:seq<Packet>) 
+    requires pkt.msg.Accept?
+    requires l.state == P2b
+{
+    var src, msg := pkt.src, pkt.msg;
+    if msg.bal == l.ballot && src !in l.accepts then
+        LeaderProcessValidAccept(l, l', src, msg, sendIos)
+    else 
+        // This is a stale Accept
+        LeaderStutter(l, l', sendIos)
+}
+
+predicate LeaderProcessValidAccept(l:Leader, l':Leader, src:Id, msg:Message, sendIos:seq<Packet>) 
+    requires msg.Accept?
+    requires l.state == P2b
+{
+    if |l.accepts| == 2*l.consts.f then 
+        // Go to Decided state
+        && l'.state == Decided
+        && l'.ballot == l.ballot
+        && l'.val == l.val
+        && l'.promises == l.promises
+        && l'.accepts == l.accepts
+    else 
+        && l'.state == l.state
+        && l'.ballot == l.ballot
+        && l'.val == l.val
+        && l'.promises == l.promises
+        && l'.accepts == l.accepts + {src}
+}
 }
