paxos/types.dfy
@@ -8,9 +8,9 @@ datatype Value = V(val:int) | Nil
 datatype Ballot = Ballot(seqNo:nat, num:nat) | Bottom
 
 datatype Message = Prepare(bal:Ballot)
-                | Promise(val:Value)
+                | Promise(bal:Ballot, val:Value)
                 | Propose(bal:Ballot, val:Value)
-                | Accept()
+                | Accept(bal:Ballot)
                 | Preempt(bal:Ballot, val:Value)
 
 datatype Packet = Packet(src:Id, dst:Id, msg:Message)
@@ -29,6 +29,21 @@ predicate BalLt(b1:Ballot, b2:Ballot) {
 /* True iff b1 <= b2 */
 predicate BalLtEq(b1:Ballot, b2:Ballot) {
     b1 == b2 || BalLt(b1, b2)
+}
+
+/* True iff b1 > b2 */
+predicate BalGt(b1:Ballot, b2:Ballot) {
+    !BalLtEq(b1, b2)
+}
+
+/* Returns the next largest ballot for non-Bottom ballots, belonging to a given leader num */
+function {:opaque} NextBallot(b:Ballot, num:nat) : (b':Ballot) 
+    ensures b != Bottom ==> b' != Bottom
+    ensures b != Bottom ==> BalGt(b', b)
+    ensures b != Bottom ==> b'.num == num
+{
+    if b == Bottom then Bottom
+    else Ballot(b.seqNo + 1, num)
 }
 
 
